Finally figured out how to do bidirectional typechecking with inferred and checked terms defined by mutual induction. Used this for a checker/inferencer for STLC with empty, unit, pairs and sums.

Lambda/Bidirectional.v
@@ -156,6 +156,9 @@ with check_type : Ctx -> tm -> type -> Prop :=
         forall (G : Ctx) (t : tm) (A : type),
           infer_type G t A -> check_type G t A.
 
+Hint Constructors infer_type.
+Hint Constructors check_type.
+
 Fixpoint type_eq_dec (t1 t2 : type) : bool :=
 match t1, t2 with
     | TBool, TBool => true
@@ -247,7 +250,8 @@ Proof.
   destruct t; cbn; intros.
     constructor. assumption.
     case_eq (infer G t1); intros; rewrite H0 in H.
-      destruct t; inv H. case_eq (check G t2 t3); intro; rewrite H in H2; inv H2.
+      destruct t; inv H.
+      case_eq (check G t2 t3); intro; rewrite H in H2; inv H2.
         eapply infer_App.
           eapply infer_correct. exact H0.
           apply check_correct. assumption.
@@ -258,7 +262,8 @@ Proof.
     case_eq (G v); intros; rewrite H0 in H; inv H.
       apply type_eq_dec_true in H2; subst. do 2 constructor. assumption.
     case_eq (infer G t1); intros; rewrite H0 in H.
-      destruct t; inv H. case_eq (check G t2 t3); intro; rewrite H in H2; inv H2.
+      destruct t; inv H.
+      case_eq (check G t2 t3); intro; rewrite H in H2; inv H2.
         apply type_eq_dec_true in H3; subst.
           constructor. eapply infer_App.
             apply infer_correct. exact H0.
@@ -266,10 +271,11 @@ Proof.
       congruence.
     1-3: destruct A; inversion H.
       constructor. apply check_correct. assumption.
-      do 2 constructor.
-      do 2 constructor.
+    do 2 constructor.
+    do 2 constructor.
     constructor; apply check_correct;
-      destruct (check G t1 TBool), (check G t2 A), (check G t3 A); cbn in H; auto.
+      destruct (check G t1 TBool), (check G t2 A), (check G t3 A);
+        cbn in H; auto.
     constructor. case_eq (check G t t0); intros; rewrite H0 in H; inv H.
       apply type_eq_dec_true in H2; subst. constructor.
         apply check_correct. assumption.
@@ -295,3 +301,557 @@ Proof.
 Qed.
 
 End Bidirectional_STLC_with_Booleans.
+
+(** 1.3 Bidirectional STLC with Booleans using mutual induction *)
+
+Module Bidirectional_STLC_with_Booleans_using_mutual_induction.
+
+Parameter V : Type.
+Parameter dec : V -> V -> bool.
+Parameter dec_spec :
+  forall x y : V, reflect (x = y) (dec x y).
+
+Notation "x =? y" := (dec x y) (at level 70).
+
+Inductive type : Type :=
+    | TBool : type
+    | TArr : type -> type -> type.
+
+Inductive tmEx : Type :=
+    | TVar : V -> tmEx
+    | TApp : tmEx -> tmIn -> tmEx
+    | TTrue : tmEx
+    | TFalse : tmEx
+    | TAnn : tmIn -> type -> tmEx
+
+with tmIn : Type :=
+    | TLam : V -> tmIn -> tmIn
+    | TIf : tmIn -> tmIn -> tmIn -> tmIn
+    | TEx : tmEx -> tmIn.
+
+Definition Ctx : Type := V -> option type.
+
+Inductive infer_type : Ctx -> tmEx -> type -> Prop :=
+    | infer_Var :
+        forall (G : Ctx) (x : V) (A : type),
+          G x = Some A -> infer_type G (TVar x) A
+    | infer_App :
+        forall (G : Ctx) (t1 : tmEx) (t2 : tmIn) (A B : type),
+          infer_type G t1 (TArr A B) -> check_type G t2 A ->
+            infer_type G (TApp t1 t2) B
+    | infer_True :
+        forall G : Ctx, infer_type G TTrue TBool
+    | infer_False :
+        forall G : Ctx, infer_type G TFalse TBool
+    | infer_Ann :
+        forall (G : Ctx) (t : tmIn) (A : type),
+          check_type G t A -> infer_type G (TAnn t A) A
+
+with check_type : Ctx -> tmIn -> type -> Prop :=
+    | check_Lam :
+        forall (G : Ctx) (x : V) (t : tmIn) (A B : type),
+          check_type (fun v : V => if x =? v then Some A else G v) t B ->
+            check_type G (TLam x t) (TArr A B)
+    | check_If :
+        forall (G : Ctx) (t1 t2 t3 : tmIn) (A : type),
+          check_type G t1 TBool -> check_type G t2 A -> check_type G t3 A ->
+            check_type G (TIf t1 t2 t3) A
+    | check_Ex :
+        forall (G : Ctx) (t : tmEx) (A : type),
+          infer_type G t A -> check_type G (TEx t) A.
+
+Hint Constructors infer_type.
+Hint Constructors check_type.
+
+Fixpoint type_eq_dec (t1 t2 : type) : bool :=
+match t1, t2 with
+    | TBool, TBool => true
+    | TArr t11 t12, TArr t21 t22 =>
+        type_eq_dec t11 t21 && type_eq_dec t12 t22
+    | _, _ => false
+end.
+
+Fixpoint infer (G : Ctx) (t : tmEx) : option type :=
+match t with
+    | TVar x => G x
+    | TApp t1 t2 =>
+        match infer G t1 with
+            | Some (TArr A B) => if check G t2 A then Some B else None
+            | _ => None
+        end
+    | TTrue => Some TBool
+    | TFalse => Some TBool
+    | TAnn t A => if check G t A then Some A else None
+end
+
+with check (G : Ctx) (t : tmIn) (A : type) : bool :=
+match t with
+    | TLam x t =>
+        match A with
+            | TArr X Y =>
+                check (fun v : V => if x =? v then Some X else G v) t Y
+            | _ => false
+        end
+    | TIf t1 t2 t3 =>
+        check G t1 TBool && check G t2 A && check G t3 A
+    | TEx t' =>
+        match infer G t' with
+            | Some B => type_eq_dec A B
+            | _ => false
+        end
+end.
+
+Lemma type_eq_dec_refl :
+  forall A : type, type_eq_dec A A = true.
+Proof.
+  induction A; cbn.
+    reflexivity.
+    rewrite IHA1, IHA2. cbn. reflexivity.
+Qed.
+
+Lemma type_eq_dec_true :
+  forall A B : type,
+    type_eq_dec A B = true -> A = B.
+Proof.
+  induction A; destruct B; cbn; intros; try congruence.
+  specialize (IHA1 B1). specialize (IHA2 B2).
+  destruct (type_eq_dec A1 B1), (type_eq_dec A2 B2).
+    all: firstorder; congruence.
+Qed.
+
+Ltac inv H := inversion H; subst; clear H.
+
+Lemma infer_correct :
+  forall (G : Ctx) (t : tmEx) (A : type),
+    infer G t = Some A -> infer_type G t A
+
+with check_correct :
+  forall (G : Ctx) (t : tmIn) (A : type),
+    check G t A = true -> check_type G t A.
+Proof.
+  destruct t; cbn; intros.
+    constructor. assumption.
+    case_eq (infer G t); intros; rewrite H0 in H.
+      destruct t1; inv H.
+      case_eq (check G t0 t1_1); intro; rewrite H in H2; inv H2.
+      eapply infer_App.
+        eapply infer_correct. exact H0.
+        apply check_correct. assumption.
+      inv H.
+    inv H. constructor.
+    inv H. constructor.
+    case_eq (check G t t0); intro; rewrite H0 in H; inv H.
+      constructor. apply check_correct. assumption.
+  destruct t; cbn; intros.
+    destruct A.
+      inv H.
+      constructor. apply check_correct. assumption.
+    constructor; apply check_correct;
+      destruct (check G t1 TBool), (check G t2 A), (check G t3 A); cbn in H;
+      congruence.
+    constructor. apply infer_correct. destruct (infer G t).
+      f_equal. symmetry. apply type_eq_dec_true. assumption.
+      inv H.
+Qed.
+
+Lemma infer_complete :
+  forall (G : Ctx) (t : tmEx) (A : type),
+    infer_type G t A -> infer G t = Some A
+
+with check_complete :
+  forall (G : Ctx) (t : tmIn) (A : type),
+    check_type G t A -> check G t A = true.
+Proof.
+  destruct 1; cbn; intros.
+    assumption.
+    rewrite (infer_complete _ _ _ H), (check_complete _ _ _ H0). reflexivity.
+    1-2: reflexivity.
+    rewrite (check_complete _ _ _ H). reflexivity.
+  destruct 1; cbn; intros.
+    apply check_complete. assumption.
+    rewrite !check_complete; cbn; auto.
+    rewrite (infer_complete _ _ _ H). apply type_eq_dec_refl.
+Qed.
+
+End Bidirectional_STLC_with_Booleans_using_mutual_induction.
+
+(** 1.4 Bidirectional STLC with lots of other stuff *)
+
+Module Bidirectional_STLC_with_stuff.
+
+Parameter V : Type.
+Parameter dec : V -> V -> bool.
+Parameter dec_spec :
+  forall x y : V, reflect (x = y) (dec x y).
+
+Notation "x =? y" := (dec x y) (at level 70).
+
+Inductive type : Type :=
+    | TArr : type -> type -> type
+    | TEmpty : type
+    | TUnit : type
+    | TBool : type
+    | TProd : type -> type -> type
+    | TSum : type -> type -> type.
+
+Inductive tmEx : Type :=
+    | TVar : V -> tmEx
+    | TAnn : tmIn -> type -> tmEx
+
+    | TApp : tmEx -> tmIn -> tmEx
+
+    | TStar : tmEx
+
+    | TTrue : tmEx
+    | TFalse : tmEx
+    | TIf : tmIn -> tmEx -> tmEx -> tmEx
+
+    | TPair : tmEx -> tmEx -> tmEx
+    | TOutl : tmEx -> tmEx
+    | TOutr : tmEx -> tmEx
+
+    | TCase : tmEx -> tmEx -> tmEx -> tmEx
+
+with tmIn : Type :=
+    | TEx : tmEx -> tmIn
+    | TLam : V -> tmIn -> tmIn
+    | TExfalso : tmIn -> tmIn
+(*    | TExfalso : tmIn -> type -> tmIn *)
+
+    | TInl : tmIn -> tmIn
+    | TInr : tmIn -> tmIn.
+
+(*  | TCase *)
+
+Definition Ctx : Type := V -> option type.
+
+Inductive infer_type : Ctx -> tmEx -> type -> Prop :=
+    | infer_Var :
+        forall (G : Ctx) (x : V) (A : type),
+          G x = Some A -> infer_type G (TVar x) A
+    | infer_Ann :
+        forall (G : Ctx) (t : tmIn) (A : type),
+          check_type G t A -> infer_type G (TAnn t A) A
+    | infer_App :
+        forall (G : Ctx) (t1 : tmEx) (t2 : tmIn) (A B : type),
+          infer_type G t1 (TArr A B) -> check_type G t2 A ->
+            infer_type G (TApp t1 t2) B
+    | infer_Star :
+        forall G : Ctx, infer_type G TStar TUnit
+    | infer_True :
+        forall G : Ctx, infer_type G TTrue TBool
+    | infer_False :
+        forall G : Ctx, infer_type G TFalse TBool
+    | infer_If :
+        forall (G : Ctx) (t1 : tmIn) (t2 t3 : tmEx) (A : type),
+          check_type G t1 TBool ->
+          infer_type G t2 A -> infer_type G t3 A ->
+            infer_type G (TIf t1 t2 t3) A
+    | infer_Pair :
+        forall (G : Ctx) (t1 t2 : tmEx) (A B : type),
+          infer_type G t1 A -> infer_type G t2 B ->
+            infer_type G (TPair t1 t2) (TProd A B)
+    | infer_Outl :
+        forall (G : Ctx) (t : tmEx) (A B : type),
+          infer_type G t (TProd A B) -> infer_type G (TOutl t) A
+    | infer_Outr :
+        forall (G : Ctx) (t : tmEx) (A B : type),
+          infer_type G t (TProd A B) -> infer_type G (TOutr t) B
+    | infer_Case :
+        forall (G : Ctx) (t1 t2 t3 : tmEx) (A B C : type),
+          infer_type G t1 (TSum A B) ->
+          infer_type G t2 (TArr A C) ->
+          infer_type G t3 (TArr B C) ->
+            infer_type G (TCase t1 t2 t3) C
+
+with check_type : Ctx -> tmIn -> type -> Prop :=
+    | check_Ex :
+        forall (G : Ctx) (t : tmEx) (A : type),
+          infer_type G t A -> check_type G (TEx t) A
+    | check_Lam :
+        forall (G : Ctx) (x : V) (t : tmIn) (A B : type),
+          check_type (fun v : V => if x =? v then Some A else G v) t B ->
+            check_type G (TLam x t) (TArr A B)
+(*    | check_Exfalso :
+        forall (G : Ctx) (t : tmIn) (A : type),
+          check_type G t TEmpty -> check_type G (TExfalso t A) A *)
+    | check_Exfalso :
+        forall (G : Ctx) (t : tmIn) (A : type),
+          check_type G t TEmpty -> check_type G (TExfalso t) A
+    | check_Inl :
+        forall (G : Ctx) (t : tmIn) (A B : type),
+          check_type G t A -> check_type G (TInl t) (TSum A B)
+    | check_Inr :
+        forall (G : Ctx) (t : tmIn) (A B : type),
+          check_type G t B -> check_type G (TInr t) (TSum A B).
+
+Hint Constructors infer_type.
+Hint Constructors check_type.
+
+Print type.
+
+Fixpoint type_eq_dec (t1 t2 : type) : bool :=
+match t1, t2 with
+    | TArr t11 t12, TArr t21 t22 =>
+        type_eq_dec t11 t21 && type_eq_dec t12 t22
+    | TEmpty, TEmpty => true
+    | TUnit, TUnit => true
+    | TBool, TBool => true
+    | TProd t11 t12, TProd t21 t22 =>
+        type_eq_dec t11 t21 && type_eq_dec t12 t22
+    | TSum t11 t12, TSum t21 t22 =>
+        type_eq_dec t11 t21 && type_eq_dec t12 t22
+    | _, _ => false
+end.
+
+Require Import Bool.
+
+Lemma type_eq_dec_spec :
+  forall A B : type, reflect (A = B) (type_eq_dec A B).
+Proof.
+  induction A; destruct B; cbn; try constructor; try inversion 1.
+    destruct (IHA1 B1), (IHA2 B2); cbn; constructor; congruence.
+    1-3: reflexivity.
+    destruct (IHA1 B1), (IHA2 B2); cbn; constructor; congruence.
+    destruct (IHA1 B1), (IHA2 B2); cbn; constructor; congruence.
+Qed.
+
+Print tmEx.
+
+Fixpoint infer (G : Ctx) (t : tmEx) : option type :=
+match t with
+    | TVar x => G x
+    | TAnn t A => if check G t A then Some A else None
+    | TApp t1 t2 =>
+        match infer G t1 with
+            | Some (TArr A B) => if check G t2 A then Some B else None
+            | _ => None
+        end
+    | TStar => Some TUnit
+    | TTrue => Some TBool
+    | TFalse => Some TBool
+    | TIf t1 t2 t3 =>
+        match infer G t2, infer G t3 with
+            | Some A, Some B =>
+                if check G t1 TBool && type_eq_dec A B then Some A else None
+            | _, _ => None
+        end
+    | TPair t1 t2 =>
+        match infer G t1, infer G t2 with
+            | Some A, Some B => Some (TProd A B)
+            | _, _ => None
+        end
+    | TOutl t' =>
+        match infer G t' with
+            | Some (TProd A B) => Some A
+            | _ => None
+        end
+    | TOutr t' =>
+        match infer G t' with
+            | Some (TProd A B) => Some B
+            | _ => None
+        end
+    | TCase t1 t2 t3 =>
+        match infer G t1, infer G t2, infer G t3 with
+            | Some (TSum A B), Some (TArr A' C), Some (TArr B' C') =>
+                if
+                  type_eq_dec A A' &&
+                  type_eq_dec B B' &&
+                  type_eq_dec C C'
+                then
+                  Some C
+                else None
+            | _, _, _ => None
+        end
+end
+
+with check (G : Ctx) (t : tmIn) (A : type) : bool :=
+match t with
+    | TEx t' =>
+        match infer G t' with
+            | Some B => type_eq_dec A B
+            | _ => false
+        end
+    | TLam x t =>
+        match A with
+            | TArr X Y =>
+                check (fun v : V => if x =? v then Some X else G v) t Y
+            | _ => false
+        end
+(*    | TExfalso t' B => check G t' TEmpty && type_eq_dec A B *)
+    | TExfalso t' => check G t' TEmpty
+    | TInl t' =>
+        match A with
+            | TSum B C => check G t' B
+            | _ => false
+        end
+    | TInr t' =>
+        match A with
+            | TSum B C => check G t' C
+            | _ => false
+        end
+end.
+
+Ltac inv H := inversion H; subst; clear H.
+
+Lemma infer_correct :
+  forall (G : Ctx) (t : tmEx) (A : type),
+    infer G t = Some A -> infer_type G t A
+
+with check_correct :
+  forall (G : Ctx) (t : tmIn) (A : type),
+    check G t A = true -> check_type G t A.
+Proof.
+  destruct t; cbn; intros.
+    constructor. assumption.
+    case_eq (check G t t0); intro H'; rewrite H' in H; inv H.
+      constructor. apply check_correct. assumption.
+    case_eq (infer G t).
+      intros C H'. rewrite H' in H. destruct C as []; inv H.
+        case_eq (check G t0 C1); intro H''; rewrite H'' in H1; inv H1.
+        econstructor.
+          apply infer_correct. exact H'.
+          apply check_correct. assumption.
+      intro H'. rewrite H' in H. inv H.
+    1-3: inv H; constructor.
+    case_eq (infer G t2); [intros t H' | intro H']; rewrite H' in H; inv H.
+      case_eq (infer G t3); [intros t' H'' | intro H''];
+      rewrite H'' in H1; inv H1.
+      case_eq (check G t1 TBool); intro H'''; rewrite H''' in H0; inv H0.
+      destruct (type_eq_dec_spec t t'); subst; inv H1. auto.
+    case_eq (infer G t1); intros; rewrite H0 in *; inv H.
+      case_eq (infer G t2); intros; rewrite H in *; inv H2.
+      auto.
+    case_eq (infer G t); intros; rewrite H0 in *; inv H.
+      destruct t0; inv H2. econstructor. apply infer_correct.
+      cbn. rewrite H0. reflexivity.
+    case_eq (infer G t); intros; rewrite H0 in *; inv H.
+      destruct t0; inv H2. econstructor. apply infer_correct.
+      cbn. rewrite H0. reflexivity.
+    case_eq (infer G t1); intros; rewrite H0 in *; try destruct t; inv H.
+      case_eq (infer G t2); intros; rewrite H in *; try destruct t; inv H2.
+      case_eq (infer G t3); intros; rewrite H1 in *; try destruct t; inv H3.
+      destruct
+        (type_eq_dec_spec t4 t6),
+        (type_eq_dec_spec t5 t8),
+        (type_eq_dec_spec t7 t9);
+      cbn in *; subst; inv H4; try congruence.
+      econstructor; apply infer_correct; eassumption.
+  destruct t; cbn; intros.
+    constructor. apply infer_correct. destruct (infer G t).
+      f_equal. destruct (type_eq_dec_spec A t0); congruence.
+      inv H.
+    destruct A; inv H. constructor. apply check_correct. assumption.
+(*
+    destruct (type_eq_dec_spec A t0); subst.
+      constructor. apply check_correct. rewrite andb_true_r in H. assumption.
+      rewrite andb_false_r in H. inv H.
+*)
+    constructor. apply check_correct. assumption.
+    destruct A; inv H. constructor. apply check_correct. assumption.
+    destruct A; inv H. constructor. apply check_correct. assumption.
+Qed.
+
+Lemma infer_correct'' :
+  forall (G : Ctx) (t : tmEx) (A : type),
+    infer G t = Some A <-> infer_type G t A
+
+with check_correct'' :
+  forall (G : Ctx) (t : tmIn) (A : type),
+    reflect (check_type G t A) (check G t A).
+Proof.
+  split.
+    destruct t; cbn; intros.
+      constructor. assumption.
+      destruct (check_correct'' G t t0); inv H. constructor. assumption.
+      case_eq (infer G t).
+        intros C H'. rewrite H' in H. destruct C as []; inv H.
+          case_eq (check G t0 C1); intro H''; rewrite H'' in H1; inv H1.
+          econstructor.
+            apply infer_correct. exact H'.
+            apply check_correct. assumption.
+        intro H'. rewrite H' in H. inv H.
+      1-3: inv H; constructor.
+      case_eq (infer G t2); intros; rewrite H0 in H; inv H.
+        case_eq (infer G t3); intros; rewrite H in H2; inv H2.
+        destruct (check_correct'' G t1 TBool); inv H3.
+        destruct (type_eq_dec_spec t t0); inv H2.
+        constructor.
+          assumption.
+          1-2: apply infer_correct; assumption.
+      case_eq (infer G t1); intros; rewrite H0 in *; inv H.
+        case_eq (infer G t2); intros; rewrite H in *; inv H2.
+        constructor; rewrite <- infer_correct''; assumption.
+      case_eq (infer G t); intros; rewrite H0 in *; inv H.
+        destruct t0; inv H2. econstructor. apply infer_correct.
+        cbn. rewrite H0. reflexivity.
+      case_eq (infer G t); intros; rewrite H0 in *; inv H.
+        destruct t0; inv H2. econstructor. apply infer_correct.
+        cbn. rewrite H0. reflexivity.
+      case_eq (infer G t1); intros; rewrite H0 in *; try destruct t; inv H.
+        case_eq (infer G t2); intros; rewrite H in *; try destruct t; inv H2.
+        case_eq (infer G t3); intros; rewrite H1 in *; try destruct t; inv H3.
+        destruct
+          (type_eq_dec_spec t4 t6),
+          (type_eq_dec_spec t5 t8),
+          (type_eq_dec_spec t7 t9);
+        cbn in *; subst; inv H4; try congruence.
+        econstructor; apply infer_correct; eassumption.
+    destruct t; cbn; intro H; inv H.
+      assumption.
+      destruct (check_correct'' G t A).
+        reflexivity.
+        contradiction.
+      destruct (infer_correct'' G t (TArr A0 A)).
+        rewrite (H0 H3). destruct (check_correct'' G t0 A0); subst.
+          reflexivity.
+          contradiction.
+      1-3: reflexivity.
+      destruct (infer_correct'' G t2 A), (infer_correct'' G t3 A).
+        rewrite (H0 H6), (H2 H7).
+        destruct (check_correct'' G t1 TBool); subst.
+          cbn. destruct (type_eq_dec_spec A A); congruence.
+          contradiction.
+      destruct (infer_correct'' G t1 A0), (infer_correct'' G t2 B).
+        rewrite (H0 H3), (H2 H5). reflexivity.
+      destruct (infer_correct'' G t (TProd A B)).
+        rewrite (H0 H2). reflexivity.
+      destruct (infer_correct'' G t (TProd A0 A)).
+        rewrite (H0 H2). reflexivity.
+      destruct
+            (infer_correct'' G t1 (TSum A0 B)),
+            (infer_correct'' G t2 (TArr A0 A)),
+            (infer_correct'' G t3 (TArr B A)).
+        rewrite (H0 H4), (H2 H6), (H5 H7).
+        destruct
+          (type_eq_dec_spec A0 A0),
+          (type_eq_dec_spec B B),
+          (type_eq_dec_spec A A); subst; cbn; congruence.
+  destruct t; cbn; intros.
+    case_eq (infer G t); intros.
+      destruct (type_eq_dec_spec A t0); constructor; subst.
+        constructor. apply infer_correct. assumption.
+        intro. inv H0. destruct (infer_correct'' G t A).
+          specialize (H1 H3). congruence.
+      constructor. intro. inv H0. destruct (infer_correct'' G t A).
+        specialize (H1 H3). congruence.
+    destruct A; try constructor; try inversion 1.
+      destruct (check_correct''
+        (fun v0 : V => if v =? v0 then Some A1 else G v0) t A2);
+      constructor.
+        constructor. assumption.
+        intro. inv H. contradiction.
+    destruct (check_correct'' G t TEmpty); subst; constructor.
+      constructor. assumption.
+      intro. inv H. contradiction.
+    destruct A; try constructor; try inversion 1.
+      destruct (check_correct'' G t A1); constructor.
+        constructor. assumption.
+        intro. inv H. contradiction.
+    destruct A; try constructor; try inversion 1.
+      destruct (check_correct'' G t A2); constructor.
+        constructor. assumption.
+        intro. inv H. contradiction.
+Qed.
+
+End Bidirectional_STLC_with_stuff.
